week5/mirror-submission.dfy
@@ -1,8 +1,8 @@
 // BEGIN-TODO(Name)
 // Please, before you do anything else, add your names here:
-// Group <Group number>
-// <Full name 1>: <Student number 1>
-// <Full name 2>: <Student number 2>
+// Group 36
+// Matilda Fogato: 1656376
+// Jip Melle Verkoulen: 1836587
 //
 // Good luck!
 //
@@ -18,8 +18,14 @@ datatype BYTree = BlueLeaf
 
 function Mirror(t: BYTree): BYTree
 {
-// BEGIN-TODO(Mirror)
-// Implement the `Mirror` predicate according to the instructions.
-// END-TODO(Mirror)
+  // BEGIN-TODO(Mirror)
+  // Implement the `Mirror` predicate according to the instructions.
+  match t
+  case BlueLeaf => BlueLeaf
+  case YellowLeaf => YellowLeaf
+  case Node(left, right) => Node(Mirror(right), Mirror(left))
+
+
+  // END-TODO(Mirror)
 }
 
