week5/swedish-color-tree-submission.dfy
@@ -1,8 +1,8 @@
 // BEGIN-TODO(Name)
 // Please, before you do anything else, add your names here:
-// Group <Group number>
-// <Full name 1>: <Student number 1>
-// <Full name 2>: <Student number 2>
+// Group 36
+// Matilda Fogato: 1656376
+// Jip Melle Verkoulen: 1836587
 //
 // Good luck!
 //
@@ -24,7 +24,13 @@ predicate IsSwedishFlagColor(c : Color)
 
 predicate IsSwedishColoredTree(t: ColoredTree)
 {
-// BEGIN-TODO(IsSwedishColorTree)
-// Implement the `IsSwedishColoredTree` predicate according to the instructions.
-// END-TODO(IsSwedishColorTree)
+  // BEGIN-TODO(IsSwedishColorTree)
+  // Define a predicate on colored trees that determines whether all leaves have colors that are part of the Swedish flag.
+  match t
+  {
+    case Leaf(c) => IsSwedishFlagColor(c)
+    case Node(left, right) => IsSwedishColoredTree(left) && IsSwedishColoredTree(right)
+  }
+
+  // END-TODO(IsSwedishColorTree)
 }
